Test/Test_regression.lean
@@ -41,6 +41,50 @@ example (as bs cs : List α) (f : α → β) :
   apply monoLem_0
   rw [monoLem_1]; rw [monoLem_3]; rw [monoLem_3]
 
+open Auto in
+set_option trace.auto.mono.printConstInst true in
+example
+  (Vector8 : Type u → Type u)
+  (map : ∀ {α} {β} (f : α → β), Vector8 α → Vector8 β)
+  (zip : ∀ {α} {β}, Vector8 α → Vector8 β → Vector8 (α × β))
+  (zip_map_prod_fst : ∀ {α} {β} (xs : Vector8 α) (ys : Vector8 β),
+    map Prod.fst (zip xs ys) = xs)
+  (zip_map_prod_snd : ∀ {α} {β} (xs : Vector8 α) (ys : Vector8 β),
+    map Prod.snd (zip xs ys) = ys)
+  (as bs cs ds : Vector8 α)
+  (h : ∀ (δ : Type _) (f₁ f₂ f₃ f₄ : δ → α) (xs : Vector8 δ),
+    map f₁ xs = as ∧ map f₂ xs = bs ∧ map f₃ xs = cs ∧ map f₄ xs = ds → False) :
+  False := by
+  -- `auto` cannot properly find the expected instantiations because
+  --   we do not collect partially instantiated polymorphic constants
+  --   (i.e. polymorphic constants with some dependent arguments instantiated
+  --    and some dependent arguments not instantiated)
+  --   and we do not match against instances of polymorphic logical constants
+  --   (i.e. `∀, ∃, =`)
+  intromono [zip_map_prod_fst, zip_map_prod_snd, h]; sorry
+
+section MonomorphizationWierdExample
+
+  def List.directZip : {α : Type u} → List α → {β : Type v} → List β → List (α × β)
+    | _, [], _, []   => []
+    | _, [], _, _::_ => []
+    | _, _::_, _, [] => []
+    | _, x::xs, _, y::ys => (x,y) :: directZip xs ys
+
+  def prod_eq₁' : ∀ (x : α) (y : β), Prod.fst (x, y) = x := sorry
+  def prod_eq₂' : ∀ (x : α) (y : β), Prod.snd (x, y) = y := sorry
+
+  set_option auto.mono.saturationThreshold 800 in
+  example
+    (α : Type u)
+    (as bs cs ds : List α)
+    (hab : as.length = bs.length) (hbc : bs.length = cs.length) (hcd : cs.length = ds.length)
+    (h : ∀ (δ : Type u) (f₁ f₂ f₃ f₄ : δ → α) (xs : List δ),
+      xs.map f₁ = as ∧ xs.map f₂ = bs ∧ xs.map f₃ = cs ∧ xs.map f₄ = ds → False) : False := by
+    intromono [h, hab, prod_eq₁', prod_eq₂'] d[List.length, List.directZip, List.map]; sorry
+
+end MonomorphizationWierdExample
+
 -- Data Structure Robustness
 
 section DSRobust
